Propagate errors up through existentials

src/MicroSail/Symbolic/Mutator.v
@@ -690,10 +690,20 @@ Module Mutators
 
   Module SPath.
 
+    Inductive EMessage (Σ : LCtx) : Type :=
+    | EMsgHere (msg : Message Σ)
+    | EMsgThere {b} (msg : EMessage (Σ ▻ b)).
+
+    Fixpoint shift_emsg {Σ b} (bIn : b ∈ Σ) (emsg : EMessage (Σ - b)) : EMessage Σ :=
+      match emsg with
+      | EMsgHere msg   => EMsgHere (subst msg (sub_shift bIn))
+      | EMsgThere emsg => EMsgThere (shift_emsg (inctx_succ bIn) emsg)
+      end.
+
     Inductive SPath (Σ : LCtx) : Type :=
     | angelic_binary (o1 o2 : SPath Σ)
     | demonic_binary (o1 o2 : SPath Σ)
-    | error (msg : Message Σ)
+    | error (msg : EMessage Σ)
     | block
     | assertk (fml : Formula Σ) (msg : Message Σ) (k : SPath Σ)
     | assumek (fml : Formula Σ) (k : SPath Σ)
@@ -975,54 +985,54 @@ Module Mutators
         intuition.
     Qed.
 
-    Fixpoint occurs_check_spath {Σ x} (xIn : x ∈ Σ) (p : SPath Σ) : option (SPath (Σ - x)) :=
-      match p with
-      | angelic_binary o1 o2 =>
-        option_ap (option_map (angelic_binary (Σ := Σ - x)) (occurs_check_spath xIn o1)) (occurs_check_spath xIn o2)
-      | demonic_binary o1 o2 =>
-        option_ap (option_map (demonic_binary (Σ := Σ - x)) (occurs_check_spath xIn o1)) (occurs_check_spath xIn o2)
-      | error msg => option_map error (occurs_check xIn msg)
-      | block => Some block
-      | assertk P msg o =>
-        option_ap (option_ap (option_map (assertk (Σ := Σ - x)) (occurs_check xIn P)) (occurs_check xIn msg)) (occurs_check_spath xIn o)
-      | assumek P o => option_ap (option_map (assumek (Σ := Σ - x)) (occurs_check xIn P)) (occurs_check_spath xIn o)
-      | angelicv b o => option_map (angelicv b) (occurs_check_spath (inctx_succ xIn) o)
-      | demonicv b o => option_map (demonicv b) (occurs_check_spath (inctx_succ xIn) o)
-      | @assert_vareq _ y σ yIn t msg o =>
-        match occurs_check_view yIn xIn with
-        | Same _ => None
-        | @Diff _ _ _ _ x xIn =>
-          option_ap
-            (option_ap
-               (option_map
-                  (fun (t' : Term (Σ - (y :: σ) - x) σ) (msg' : Message (Σ - (y :: σ) - x)) (o' : SPath (Σ - (y :: σ) - x)) =>
-                     let e := swap_remove yIn xIn in
-                     assert_vareq
-                       y
-                       (eq_rect (Σ - (y :: σ) - x) (fun Σ => Term Σ σ) t' (Σ - x - (y :: σ)) e)
-                       (eq_rect (Σ - (y :: σ) - x) Message msg' (Σ - x - (y :: σ)) e)
-                       (eq_rect (Σ - (y :: σ) - x) SPath o' (Σ - x - (y :: σ)) e))
-                  (occurs_check xIn t))
-               (occurs_check xIn msg))
-            (occurs_check_spath xIn o)
-        end
-      | @assume_vareq _ y σ yIn t o =>
-        match occurs_check_view yIn xIn with
-        | Same _ => Some o
-        | @Diff _ _ _ _ x xIn =>
-          option_ap
-            (option_map
-               (fun (t' : Term (Σ - (y :: σ) - x) σ) (o' : SPath (Σ - (y :: σ) - x)) =>
-                  let e := swap_remove yIn xIn in
-                  assume_vareq
-                    y
-                    (eq_rect (Σ - (y :: σ) - x) (fun Σ => Term Σ σ) t' (Σ - x - (y :: σ)) e)
-                    (eq_rect (Σ - (y :: σ) - x) SPath o' (Σ - x - (y :: σ)) e))
-               (occurs_check xIn t))
-            (occurs_check_spath xIn o)
-        end
-      | debug b o => option_ap (option_map (debug (Σ := Σ - x)) (occurs_check xIn b)) (occurs_check_spath xIn o)
-      end.
+    (* Fixpoint occurs_check_spath {Σ x} (xIn : x ∈ Σ) (p : SPath Σ) : option (SPath (Σ - x)) := *)
+    (*   match p with *)
+    (*   | angelic_binary o1 o2 => *)
+    (*     option_ap (option_map (angelic_binary (Σ := Σ - x)) (occurs_check_spath xIn o1)) (occurs_check_spath xIn o2) *)
+    (*   | demonic_binary o1 o2 => *)
+    (*     option_ap (option_map (demonic_binary (Σ := Σ - x)) (occurs_check_spath xIn o1)) (occurs_check_spath xIn o2) *)
+    (*   | error msg => option_map error (occurs_check xIn msg) *)
+    (*   | block => Some block *)
+    (*   | assertk P msg o => *)
+    (*     option_ap (option_ap (option_map (assertk (Σ := Σ - x)) (occurs_check xIn P)) (occurs_check xIn msg)) (occurs_check_spath xIn o) *)
+    (*   | assumek P o => option_ap (option_map (assumek (Σ := Σ - x)) (occurs_check xIn P)) (occurs_check_spath xIn o) *)
+    (*   | angelicv b o => option_map (angelicv b) (occurs_check_spath (inctx_succ xIn) o) *)
+    (*   | demonicv b o => option_map (demonicv b) (occurs_check_spath (inctx_succ xIn) o) *)
+    (*   | @assert_vareq _ y σ yIn t msg o => *)
+    (*     match occurs_check_view yIn xIn with *)
+    (*     | Same _ => None *)
+    (*     | @Diff _ _ _ _ x xIn => *)
+    (*       option_ap *)
+    (*         (option_ap *)
+    (*            (option_map *)
+    (*               (fun (t' : Term (Σ - (y :: σ) - x) σ) (msg' : Message (Σ - (y :: σ) - x)) (o' : SPath (Σ - (y :: σ) - x)) => *)
+    (*                  let e := swap_remove yIn xIn in *)
+    (*                  assert_vareq *)
+    (*                    y *)
+    (*                    (eq_rect (Σ - (y :: σ) - x) (fun Σ => Term Σ σ) t' (Σ - x - (y :: σ)) e) *)
+    (*                    (eq_rect (Σ - (y :: σ) - x) Message msg' (Σ - x - (y :: σ)) e) *)
+    (*                    (eq_rect (Σ - (y :: σ) - x) SPath o' (Σ - x - (y :: σ)) e)) *)
+    (*               (occurs_check xIn t)) *)
+    (*            (occurs_check xIn msg)) *)
+    (*         (occurs_check_spath xIn o) *)
+    (*     end *)
+    (*   | @assume_vareq _ y σ yIn t o => *)
+    (*     match occurs_check_view yIn xIn with *)
+    (*     | Same _ => Some o *)
+    (*     | @Diff _ _ _ _ x xIn => *)
+    (*       option_ap *)
+    (*         (option_map *)
+    (*            (fun (t' : Term (Σ - (y :: σ) - x) σ) (o' : SPath (Σ - (y :: σ) - x)) => *)
+    (*               let e := swap_remove yIn xIn in *)
+    (*               assume_vareq *)
+    (*                 y *)
+    (*                 (eq_rect (Σ - (y :: σ) - x) (fun Σ => Term Σ σ) t' (Σ - x - (y :: σ)) e) *)
+    (*                 (eq_rect (Σ - (y :: σ) - x) SPath o' (Σ - x - (y :: σ)) e)) *)
+    (*            (occurs_check xIn t)) *)
+    (*         (occurs_check_spath xIn o) *)
+    (*     end *)
+    (*   | debug b o => option_ap (option_map (debug (Σ := Σ - x)) (occurs_check xIn b)) (occurs_check_spath xIn o) *)
+    (*   end. *)
 
     Definition angelic_binary_prune {Σ} (p1 p2 : SPath Σ) : SPath Σ :=
       match p1 , p2 with
@@ -1057,14 +1067,10 @@ Module Mutators
     Global Arguments assumek_prune {Σ} fml p.
 
     Definition angelicv_prune {Σ} b (p : SPath (Σ ▻ b)) : SPath Σ :=
-      angelicv b p.
-      (* TODO: This does not work because of the message that is included in *)
-      (* the error. We should make it possible to "strengthen" the message by *)
-      (* adding a constructor: Message (Σ ▻ b) -> Message Σ. *)
-      (* match p with *)
-      (* | error s => error s *)
-      (* | _       => angelicv b p *)
-      (* end. *)
+      match p with
+      | error msg => error (EMsgThere msg)
+      | _         => angelicv b p
+      end.
 
     Definition demonicv_prune {Σ} b (p : SPath (Σ ▻ b)) : SPath Σ :=
       (* match @occurs_check_spath AT _ (Σ ▻ b) b inctx_zero o with *)
@@ -1087,8 +1093,7 @@ Module Mutators
     Definition assert_vareq_prune {Σ} {x σ} {xIn : x::σ ∈ Σ}
       (t : Term (Σ - (x::σ)) σ) (msg : Message (Σ - (x::σ))) (k : SPath (Σ - (x::σ))) : SPath Σ :=
       match k with
-      (* TODO: Like for angelicv *)
-      (* | error s => error s *)
+      | error emsg => error (shift_emsg xIn emsg)
       | _          => assert_vareq x t msg k
       end.
     Global Arguments assert_vareq_prune {Σ} x {σ xIn} t msg k.
@@ -1165,7 +1170,7 @@ Module Mutators
 
     Lemma prune_angelicv_sound {Σ b} (p : SPath (Σ ▻ b)) (ι : SymInstance Σ) :
       safe (angelicv_prune p) ι <-> safe (angelicv b p) ι.
-    Proof. reflexivity. Qed.
+    Proof. destruct p; cbn; auto; firstorder. Qed.
 
     Lemma prune_demonicv_sound {Σ b} (p : SPath (Σ ▻ b)) (ι : SymInstance Σ) :
       safe (demonicv_prune p) ι <-> safe (demonicv b p) ι.
@@ -1174,7 +1179,7 @@ Module Mutators
     Lemma prune_assert_vareq_sound {Σ x σ} {xIn : x::σ ∈ Σ}
       (t : Term (Σ - (x::σ)) σ) (msg : Message (Σ - (x::σ))) (p : SPath (Σ - (x::σ))) (ι : SymInstance Σ) :
       safe (assert_vareq_prune x t msg p) ι <-> safe (assert_vareq x t msg p) ι.
-    Proof. reflexivity. Qed.
+    Proof. destruct p; cbn; auto; intuition. Qed.
 
     Lemma prune_assume_vareq_sound {Σ x σ} {xIn : x::σ ∈ Σ}
       (t : Term (Σ - (x::σ)) σ) (p : SPath (Σ - (x::σ))) (ι : SymInstance Σ) :
@@ -1319,7 +1324,7 @@ Module Mutators
                  (four POST (wmultisub_sup ν) (wformulas_sup w1 fmls) tt))
         | None =>
           (* The formula is inconsistent. *)
-          error msg
+          error (EMsgHere msg)
         end.
 
     Definition assume_formulas :
@@ -1369,7 +1374,7 @@ Module Mutators
       fun w msg =>
         fix rec xs POST :=
         match xs with
-        | nil        => error msg
+        | nil        => error (EMsgHere msg)
         | cons x xs  => angelic_binary (T POST x) (rec xs POST)
         end.
 
@@ -1916,13 +1921,17 @@ Module Mutators
       (*        (ma Σ1 ζ01 pc1 δ1 h1). *)
 
       Definition error {Γ1 Γ2 A D} (func : string) (msg : string) (data:D) :
-        ⊢ SMut Γ1 Γ2 A.
-      Proof.
-        intros w POST δ h.
-        apply error.
-        apply (@MkMessage _ func msg Γ1); auto.
-        apply (wco w).
-      Defined.
+        ⊢ SMut Γ1 Γ2 A :=
+        fun w _ δ h =>
+          error
+            (EMsgHere
+               {| msg_function := func;
+                  msg_message := msg;
+                  msg_program_context := Γ1;
+                  msg_localstore := δ;
+                  msg_heap := h;
+                  msg_pathcondition := wco w
+               |}).
       Global Arguments error {_ _ _ _} func msg data {w} _ _.
 
       Definition block {Γ1 Γ2 A} :
